platform/cito/ValsStringList.v
@@ -1,0 +1,4 @@
+Require Import Locals.
+
+Definition agree_in a b := List.Forall (fun x => sel a x = sel b x).
+
